move pipe example and delete verif_struct example

kalloc/Verif_basic_allocation.v
@@ -53,6 +53,25 @@ Definition kalloc_int_array_spec : ident * funspec :=
         )
     ).
 
+Definition kalloc_write_pipe_spec : ident * funspec :=
+    DECLARE _kalloc_write_pipe
+    WITH sh : share, original_freelist_pointer:val, xx:Z, ls:list val, gv:globals
+    PRE [ ] 
+        PROP () PARAMS() GLOBALS(gv) SEP (KAF_globals gv sh ls xx original_freelist_pointer)
+    POST [ tvoid ]
+        PROP ( ) RETURN () SEP (
+            (if eq_dec original_freelist_pointer nullval then
+                KAF_globals gv  sh ls xx original_freelist_pointer *emp
+            else
+            EX next ls',
+                (!! (next :: ls' = ls) &&
+                    pipe_rep sh original_freelist_pointer *
+                    KAF_globals gv  sh ls' xx next
+            )
+            )
+        ).
+       
+
 Definition kalloc_int_array_spec_fail : ident * funspec :=
     DECLARE _kalloc_int_array
     WITH sh : share, original_freelist_pointer:val, xx:Z, ls:list val, gv:globals, n:Z
@@ -185,3 +204,25 @@ forward_call (kalloc_spec_sub KAF_APD (tarray tint n)) (gv, sh , ls, xx, origina
     }
     admit. (* this is not provable as n can be arbitrary large *)
 Abort.
+
+Lemma body_kalloc_write_pipe: semax_body KAFVprog KAFGprog f_kalloc_write_pipe kalloc_write_pipe_spec.
+Proof.
+start_function.
+forward.
+forward_call (kalloc_spec_sub KAF_APD t_struct_pipe) (gv, sh , ls, xx, original_freelist_pointer ). (* kalloc *)
+- unfold KAF_globals. entailer!. 
+- if_tac. (*destruct (eq_dec original_freelist_pointer nullval) eqn:e0.*)
+    + forward_if.
+        * rewrite H in H0; auto_contradict.
+        * forward. entailer.
+    + Intros ab. forward_if.
+        rewrite mem_mgr_split. rewrite type_kalloc_token_split. Intros. rewrite kalloc_token_sz_split.
+        Intros. 
+        rewrite memory_block_data_at_; auto. rewrite data_at__eq. Intros. forward.
+        forward. forward. forward. 
+        entailer.
+        Exists  (fst ab) (snd ab). entailer.
+        unfold KAF_globals. unfold pipe_rep.  Exists (fst (default_val t_struct_pipe)). entailer!.
+        rewrite mem_mgr_split. entailer.
+        * forward. entailer.
+Qed.
